Update LDRF-RA

src/ldrfra/LocalDRFRA.v
@@ -37,18 +37,54 @@ Require Import PFtoRA.
 Set Implicit Arguments.
 
 
-Theorem local_drf_ra
-        L s
-        (RACEFREE: RARace.racefree_syn L s):
-  behaviors SConfiguration.machine_step (Configuration.init s) <1=
-  behaviors (@OrdConfiguration.step L Ordering.acqrel) (Configuration.init s).
-Proof.
-  i.
-  specialize (PFtoRA.init_sim_conf L s). intro SIM.
-  specialize (PFtoRA.init_wf_pf L s). intro WF_PF.
-  specialize (PFtoRA.init_wf_j s). intro WF_J.
-  specialize (PFtoRA.init_wf_ra s). intro WF_RA.
-  ii. exploit (@local_DRFPF_view L); eauto.
-  { eapply PFtoRA.sim_conf_racefree; eauto. }
-  eapply PFtoRA.sim_conf_behavior; eauto.
-Qed.
+Section LocalDRFRA.
+  Variable L: Loc.t -> bool.
+
+  Definition ra_racefree (c: Configuration.t): Prop :=
+    forall c1 c2 c3
+      tid_w e_w loc from to val released ordw
+      tid_r lang st3 lc3 e4 e5
+      pf e_r releasedr ordr
+      (STEPS1: rtc (@OrdConfiguration.all_step L Ordering.acqrel) c c1)
+      (WRITE_STEP: OrdConfiguration.step L Ordering.acqrel e_w tid_w c1 c2)
+      (WRITE_EVENT: ThreadEvent.is_writing e_w = Some (loc, from, to, val, released, ordw))
+      (STEPS2: rtc (@OrdConfiguration.all_step L Ordering.acqrel) c2 c3)
+      (FIND: IdentMap.find tid_r c3.(Configuration.threads) = Some (existT _ lang st3, lc3))
+      (THREAD_STEPS: rtc (@OrdThread.all_step _ L Ordering.acqrel)
+                         (Thread.mk _ st3 lc3 c3.(Configuration.sc) c3.(Configuration.memory))
+                         e4)
+      (CONS: Local.promise_consistent e4.(Thread.local))
+      (READ_STEP: OrdThread.step L Ordering.acqrel pf e_r e4 e5)
+      (READ_EVENT: ThreadEvent.is_reading e_r = Some (loc, to, val, releasedr, ordr))
+      (LOC: L loc)
+      (HIGHER: Time.lt (e4.(Thread.local).(Local.tview).(TView.cur).(View.rlx) loc) to)
+      (ORDERING: Ordering.le ordw Ordering.strong_relaxed \/
+                 Ordering.le ordr Ordering.strong_relaxed),
+      False.
+
+  Definition ra_racefree_syn (s: Threads.syntax): Prop :=
+    ra_racefree (Configuration.init s).
+
+  Lemma racefree_implies
+        s
+        (RACEFREE: ra_racefree_syn s):
+    RARace.racefree_syn L s.
+  Proof.
+  Admitted.
+
+  Theorem local_drf_ra
+          s
+          (RACEFREE: ra_racefree_syn s):
+    behaviors SConfiguration.machine_step (Configuration.init s) <1=
+    behaviors (@OrdConfiguration.machine_step L Ordering.acqrel) (Configuration.init s).
+  Proof.
+    hexploit racefree_implies; eauto. i.
+    specialize (PFtoRA.init_sim_conf L s). intro SIM.
+    specialize (PFtoRA.init_wf_pf L s). intro WF_PF.
+    specialize (PFtoRA.init_wf_j s). intro WF_J.
+    specialize (PFtoRA.init_wf_ra s). intro WF_RA.
+    ii. exploit (@local_DRFPF_view L); eauto.
+    { eapply PFtoRA.sim_conf_racefree; eauto. }
+    eapply PFtoRA.sim_conf_behavior; eauto.
+  Qed.
+End LocalDRFRA.
